\subsection{Inverse Trigonometric Functions}
\subsubsection{Derivative of Inverse Trigonometric Functions}
\begin{tabular}{ll}

$\frac{d}{dx} ( \sin^{-1} x ) = \frac{1}{\sqrt{1 - x^2}} $ & $\frac{d}{dx} ( \cos^{-1} x ) = - \frac{1}{\sqrt{1 - x^2}},\, \{ x \in \mathbf{R}\, |  -1 < x < 1  \}$ \\

$\frac{d}{dx} ( \tan^{-1} x ) = \frac{1}{1 + x^2} $ & $\frac{d}{dx} ( \cot^{-1} x ) = - \frac{1}{1 + x^2},\, \{ x \in \mathbf{R}\, |  -\infty < x < \infty \} $ \\

$\frac{d}{dx} ( \sec^{-1} x ) = \frac{1}{| x | \sqrt{x^2 - 1}} $ & $\frac{d}{dx} ( \csc^{-1} x ) = - \frac{1}{| x |\sqrt{x^2 - 1}},\, \{ x \in \mathbf{R}\, | \ |x| > 1 \} $ \\
\end{tabular}

\subsubsection{Integrals Involving Inverse Trigonometric Functions}
\begin{align}
\int \frac{dx}{\sqrt{a^2 - x^2}} &= \sin^{-1} \frac{x}{a} + C \\
\int \frac{dx}{a^2 + x^2} &= \frac{1}{a} \tan^{-1} \frac{x}{a} + C \\
\int \frac{dx}{x\sqrt{a^2 + x^2}} &= \frac{1}{a} \sec^{-1} \left| \frac{x}{a} \right| + C
\end{align}
