\subsection{Basic Approaches}

\begin{align}
\int k\, dx = & kx + C \\
\int k^p\, dx &= \frac{k^{p+1}}{p + 1} + C, p \in \mathbf{R} \ \wedge \neq -1 \\
\int \cos ax \, dx &= \frac{1}{a} \sin ax + C \\
\int \sin ax \, dx &= - \frac{1}{a} \cos ax + C \\
\int \sec^2 ax \, dx &= \frac{1}{a} \tan ax + C \\
\int \csc^2 ax \, dx &= - \frac{1}{a} \cot ax + C \\
\int \sec ax \tan ax \, dx &= \frac{1}{a} \sec ax + C \\
\int \csc ax \cot ax \, dx &= - \frac{1}{a} \csc ax \cot ax + C \\
\int e^{ax}\, dx &= \frac{1}{a} e^{ax} + C \\
\int \frac{dx}{x} &= \ln \left| x \right| + C \\
\int \frac{dx}{\sqrt{a^2 - x^2}} &= \sin^{-1} \frac{x}{a} + C \\
\int \frac{dx}{a^2 + x^2} &= \frac{1}{a} \tan^{-1} \frac{x}{a} + C \\
\int  \frac{dx}{x\sqrt{x^2 - a^2}} &= \frac{1}{a} \sec^{-1} \left| \frac{x}{a} \right| + C
\end{align}
