
\subsection{The Chain Rule}

\subsubsection{Chain Rule (One Independent Variable)}
Let $z$ be a differentiable function of $x$ and $y$ on its domain, where $x$ and $y$ are differentiable functions of $t$ on an interval $I$. Then

\begin{equation}
    \frac{dz}{dt} = \frac{\partial z}{\partial x} \frac{dx}{dt} + \frac{\partial z}{\partial y} \frac{dy}{dt}.
\end{equation}

\subsubsection{Chain Rule (Two Independent Variables)}
Let $z$ be a differentiable function of $x$ and $y$, where $x$ and $y$ are differentiable functions of $s$ and $t$. Then

\begin{equation}
    \frac{dz}{ds} = \frac{\partial z}{\partial x} \frac{\partial x}{\partial s} + \frac{\partial z}{\partial y} \frac{\partial y}{\partial s} \quad \text{and} \quad
    \frac{dz}{dt} = \frac{\partial z}{\partial x} \frac{\partial x}{\partial t} + \frac{\partial z}{\partial y} \frac{\partial y}{\partial t}
\end{equation}

\begin{multicols}{2}
\begin{forest}
for tree={ l sep=40pt,s sep=40pt,}
[z
    [x, edge=red, edge label={node[midway,left] {$\frac{\partial z}{\partial x}$}}
        [s, edge=red, edge label={node[midway,left] {$\frac{\partial x}{\partial s}$}}]
        [t, edge label={node[midway,left] {$\frac{\partial x}{\partial t}$}}]
    ]
    [y, edge=red, edge label={node[midway,left] {$\frac{\partial z}{\partial y}$}}
        [s, edge=red, edge label={node[midway,left] {$\frac{\partial y}{\partial s}$}}]
        [t, edge label={node[midway,left] {$\frac{\partial y}{\partial t}$}}]
    ]
]
\end{forest}

\begin{forest}
for tree={ l sep=40pt,s sep=40pt,}
[z
    [x, edge=red, edge label={node[midway,left] {$\frac{\partial z}{\partial x}$}}
        [s, edge label={node[midway,left] {$\frac{\partial x}{\partial s}$}}]
        [t, edge=red, edge label={node[midway,left] {$\frac{\partial x}{\partial t}$}}]
    ]
    [y, edge=red, edge label={node[midway,left] {$\frac{\partial z}{\partial y}$}}
        [s, edge label={node[midway,left] {$\frac{\partial y}{\partial s}$}}]
        [t, edge=red, edge label={node[midway,left] {$\frac{\partial y}{\partial t}$}}]
    ]
]
\end{forest}
\end{multicols}

\subsubsection{Implicit Differentiation}
Let $F$ be differentiable on its domain and suppose that $F(x,\, y) = 0$ defines $y$ as a differentiable function of $x$. Provided $F_y \neq 0$.

\begin{equation}
    \frac{dy}{dx} = - \frac{F_x}{F_y}
\end{equation}
