\RequirePackage[l2tabu, orthodox]{nag}
\documentclass[11pt]{article}

\usepackage{amssymb,amsmath,verbatim,graphicx,microtype,upquote,units,booktabs,akkwidepage}
\usepackage[margin=10pt, font=small, labelfont=bf, labelsep=endash]{caption}
\usepackage[utf8]{inputenc}

\title{Numerical Methods Equations}
\date{\today}
\author{Illya Starikov}

\begin{document}
\maketitle

\section{Taylor Series}
\begin{align}
    f(a) + f'(a)(x - a) + \frac{f''(a)}{2!}(x - a)^2 + \frac{f^{(3)}(a)}{3!}(x - a)^3 + \cdots & \\ = \sum ^{\infty} _{k = 0} \frac{f^{(k)}(a)}{k!}(x - a)^k.
\end{align}

\section{Taylor Series of $e^x$}
\begin{align}
    e^x &= 1 + x + \frac{x^2}{2!} + \cdots \\
    \frac{1}{e^{-x}} &= \frac{1}{1 - x + \frac{x^2}{2} +\cdots }
\end{align}


\section{False Position}
\begin{equation}
    r = b - \frac{(b - a) \cdot f(b)}{f(b) - f(a)}
\end{equation}

\section{Newton's Method}
\begin{equation}
    x_{n + 1} = x_n + \frac{f(x_n)}{f'(x_n)}
\end{equation}


\section{Secant Lines}
\begin{equation}
    x_3 = x_1 - \frac{(x_2 - x_1) \cdot f(x_1)}{f(x_2) - f(x_1)}
\end{equation}

\section{Modified Secant Method}
\begin{equation}
    x_2 = x_1 - \frac{f(x_1) \Delta}{f(x_1+\Delta) - f(x_1)}
\end{equation}

\end{document}