\documentclass[12pt]{document}
\begin{document}


**Theorem 5.3.1**
For all integers $$ n ≥ 0, 2^{2n} - 1 $$ is divisible by 3.

**Proof**
Let the property $$ P(n) $$ be the sentence $$ ``2^{2n} - 1 is divisible by 3. ''$$

$$ 2^{2n} - 1 is divisible by 3. $$

**Show that $$ P(0) $$ is true**:
To establish $$ P(0) $$, we must show that

$$ 2^{2 * 0} -1 $$ is divisible 3.

But

$$ 2^{2*0} - 1 = 2^0 - 1 = 1 - 1 = 0 $$

and 0 is divisible by 3 because $$ 0 = 3 * 0 $$. Hence $$ P(0) $$ is true.

**Show that for all intergers $ k ≥ 0 $, if $P(k)$ is true then $P(k + 1)$ is also true.

\end{document}